more ebpf examples

compiler_test/beepl_test/ebpf_beepl_c/BeePL_bpf_xdp_packet_count1.c
@@ -1,0 +1,64 @@
+struct xdp_md;
+struct xdp_md {
+  unsigned int data;
+  unsigned int data_end;
+  unsigned int data_meta;
+  unsigned int ingress_ifindex;
+  unsigned int rx_queue_index;
+  unsigned int egress_ifindex;
+};
+
+extern unsigned int val;
+
+extern unsigned int *counter;
+
+extern int xdp_packet_count(struct xdp_md *);
+
+extern unsigned int __compcert_va_int32(void *);
+
+extern unsigned long long __compcert_va_int64(void *);
+
+extern double __compcert_va_float64(void *);
+
+extern void *__compcert_va_composite(void *, unsigned long long);
+
+extern long long __compcert_i64_dtos(double);
+
+extern unsigned long long __compcert_i64_dtou(double);
+
+extern double __compcert_i64_stod(long long);
+
+extern double __compcert_i64_utod(unsigned long long);
+
+extern float __compcert_i64_stof(long long);
+
+extern float __compcert_i64_utof(unsigned long long);
+
+extern long long __compcert_i64_sdiv(long long, long long);
+
+extern unsigned long long __compcert_i64_udiv(unsigned long long, unsigned long long);
+
+extern long long __compcert_i64_smod(long long, long long);
+
+extern unsigned long long __compcert_i64_umod(unsigned long long, unsigned long long);
+
+extern long long __compcert_i64_shl(long long, int);
+
+extern unsigned long long __compcert_i64_shr(unsigned long long, int);
+
+extern long long __compcert_i64_sar(long long, int);
+
+extern long long __compcert_i64_smulh(long long, long long);
+
+extern unsigned long long __compcert_i64_umulh(unsigned long long, unsigned long long);
+
+unsigned int val = 0;
+
+unsigned int *counter = &val;
+
+int xdp_packet_count(struct xdp_md *ctx)
+{
+  int r;
+  *counter = *counter + 1;
+  return *counter;
+}
