compiler_test/beepl_test/BeePL_bpf_get_prandom.v
@@ -1,4 +1,4 @@
-Require Import Integers AST Ctypes BeePL BeeTypes BeePL_values BeePL_typechecker BeePL_notations. 
+Require Import Integers AST Ctypes BeePL BeeTypes BeePL_values BeePL_typechecker BeePL_notations BeePL_bpf. 
 From Coq Require Import String ZArith.
 From compcert Require Import Csyntaxdefs.
 Import Csyntaxdefs.CsyntaxNotations.
@@ -25,14 +25,7 @@ char _license[] SEC("license") = "GPL";
 Definition dattr := {| attr_volatile := false; attr_alignas := None |}.
 Definition _rand : ident := $"rand".
 Definition _bpf_get_prandom_u32 : ident := $"bpf_get_prandom_u32".
-Definition _xdp_md : ident := $"xdp_md".
 Definition _ctx : ident := $"ctx".
-Definition _data : ident := $"data".
-Definition _data_end : ident := $"data_end".
-Definition _data_meta : ident := $"data_meta".
-Definition _ingress_ifindex : ident := $"ingress_ifindex".
-Definition _rx_queue_index : ident := $"rx_queue_index".
-Definition _egress_ifindex : ident := $"egress_ifindex".
 Definition _xdp_prog : ident := $"xdp_prog".
 Definition _x : ident := $"x".
 Definition _bpf_random := $"bpf_random".
@@ -40,27 +33,13 @@ Definition _main : ident := $"main".
 Definition _h : ident := $"h". (* supposed to represent heap for Reftype *)
 
 
-Definition ident_to_string : list (ident * string) := ((_xdp_md, "xdp_md") ::
-                                                       (_ctx, "ctx") ::
+Definition ident_to_string : list (ident * string) := ident_to_string_xdp_md ++ 
+                                                      ((_ctx, "ctx") ::
                                                        (_rand, "rand") :: 
                                                        (_bpf_get_prandom_u32, "bpf_get_prandom_u32") :: 
-                                                       (_data, "data") ::
-                                                       (_data_end, "data_end") ::
-                                                       (_data_meta, "data_meta") :: 
-                                                       (_ingress_ifindex, "ingress_ifindex") ::
-                                                       (_rx_queue_index, "rx_queue_index") ::
-                                                       (_egress_ifindex, "egress_ifindex") ::
                                                        (_xdp_prog, "xdp_prog") :: 
                                                        (_x, "x") ::
                                                        (_main, "main") :: nil).
-
-Definition bpf_external_function : BeePL.external_function
-   := EF_external "bpf_get_prandom_u32" 
-      {| bsig_args := nil;
-         bsig_ef := nil;
-         bsig_res := tint32u;
-         bsig_cc := cc_default
-      |}.
 
 Definition f_xdp_prog : BeePL.function := {| 
                                    fn_return := tint32s;
@@ -72,22 +51,14 @@ Definition f_xdp_prog : BeePL.function := {|
                                    fn_body := Bind 
                                                 (_rand) tint32u
                                                 (App (Var _bpf_get_prandom_u32 (tfun nil nil tint32u)) nil tint32u)
-                                                (cint (Int.repr 1) tint32s) tint32s;
+                                                (cint (Int.repr 2) tint32s) tint32s;
                                    is_ebpf := true |}.
 
-Definition bcomposites : list bcomposite_definition :=
-(Bcomposite _xdp_md Struct
-   (Member_plain _data tint32u :: 
-    Member_plain _data_end tint32u :: 
-    Member_plain _data_meta tint32u ::
-    Member_plain _ingress_ifindex tint32u :: 
-    Member_plain _rx_queue_index tint32u :: 
-    Member_plain _egress_ifindex tint32u :: nil)
-   noattr :: nil).
+Definition bcomposites : list bcomposite_definition := bcomposites_xdp_md.
 
 
 Definition global_definitions : list (ident * AST.globdef BeePL.fundef type) 
-   := (_bpf_get_prandom_u32, AST.Gfun(BeePL.External (bpf_external_function)
+   := (_bpf_get_prandom_u32, AST.Gfun(BeePL.External bpf_get_prandom_u32
                                      nil tint32u
                                      (cc_default))) :: 
       (_xdp_prog, AST.Gfun(BeePL.Internal (f_xdp_prog))) :: nil.
