compiler_test/beepl_test/BeePL_bpf_xdp_packet_count1.v
@@ -14,7 +14,7 @@ int counter = 0;
 SEC("xdp")
 int packet_count(void *ctx) {
     counter++;
-    return XDP_PASS;
+    return *counter;
 }
 
 char LICENSE[] SEC("license") = "Dual BSD/GPL";*)
@@ -27,8 +27,6 @@ Definition _val : ident := $"val".
 Definition _ctx : ident := $"ctx".
 Definition _xdp_packet_count : ident := $"xdp_packet_count".
 Definition _main : ident := $"main".
-Definition _h : ident := $"h". (* supposed to represent heap for Reftype *)
-
 
 Definition ident_to_string : list (ident * string) := ident_to_string_xdp_md ++
                                                       ((_val, "val") ::
@@ -54,7 +52,7 @@ Definition v_counter := {|
 
 Definition f_xdp_packet_count : BeePL.function := {| 
                                    fn_return := tint32s;
-                                   fn_effect := Read mem_ident :: Write mem_ident :: nil;
+                                   fn_effect := Read mem_ident :: Write mem_ident :: Read mem_ident :: nil;
                                    fn_callconv := cc_default;
                                    fn_args := (_ctx, tpstruct _xdp_md) :: nil ;
                                    fn_vars := ((_r, tint32s) :: 
@@ -64,7 +62,7 @@ Definition f_xdp_packet_count : BeePL.function := {|
                                                                 (Prim (Bop Cop.Oadd) 
                                                                    (Prim Deref (Var _counter trint32s :: nil) tint32s ::
                                                                       cint (Int.repr 1) tint32s :: nil) tint32s) :: nil) tunit)
-                                                (cint (Int.repr 2) tint32s) tint32s;
+                                                (Prim Deref (Var _counter trint32s :: nil) tint32s) tint32s;
                                    is_ebpf := true |}.
 
 Definition bcomposites : list bcomposite_definition := bcomposites_xdp_md.
@@ -83,14 +81,14 @@ Proof.
   unfold build_bcomposite_env; simpl; constructor. 
 Qed.
 
-Definition example1 : BeePL.program := @mkbprogram bcomposites 
+(*Definition example1 : BeePL.program := @mkbprogram bcomposites 
                                                    global_definitions 
                                                    public_idents 
-                                                   _xdp_packet_count 
+                                                   _main 
                                                    bcomposite_correct
                                                    ident_to_string.
 
-(*Compute (type_check_expr example1.(prog_comp_env) 
+Compute (type_check_expr example1.(prog_comp_env) 
                          (bind_vars (bind_vars empty_context f_xdp_packet_count.(fn_args)) f_xdp_packet_count.(fn_vars)) empty_context f_xdp_packet_count.(fn_body)).
 
 
