compiler_test/beepl_test/BeePL_bpf.v
@@ -1,0 +1,143 @@
+Require Import Integers AST Ctypes BeePL BeeTypes BeePL_values BeePL_typechecker BeePL_notations. 
+From Coq Require Import String ZArith.
+From compcert Require Import Csyntaxdefs.
+Import Csyntaxdefs.CsyntaxNotations.
+Local Open Scope list_scope.
+Local Open Scope string_scope.
+Local Open Scope csyntax_scope.
+
+(***** eBPF contexts ******)
+
+Definition _pt_regs : ident := $"pt_regs".
+Definition _r15 : ident := $"r15".
+Definition _r14 : ident := $"r14".
+Definition _r13 : ident := $"r13".
+Definition _r12 : ident := $"r12".
+Definition _bp : ident := $"bp".
+Definition _bx : ident := $"bx".
+Definition _r11 : ident := $"r11".
+Definition _r10 : ident := $"r10".
+Definition _r9 : ident := $"r9".
+Definition _r8 : ident := $"r8".
+Definition _ax : ident := $"ax".
+Definition _cx : ident := $"cx".
+Definition _dx : ident := $"dx".
+Definition _si : ident := $"si".
+Definition _di : ident := $"di".
+Definition _orig_ax : ident := $"orig_ax".
+Definition _ip : ident := $"ip".
+Definition _cs : ident := $"cs".
+Definition _flags : ident := $"flags".
+Definition _sp : ident := $"sp".
+Definition _ss : ident := $"ss".
+Definition _ctx : ident := $"ctx".
+
+Definition bcomposites_pt_regs : list bcomposite_definition :=
+(Bcomposite _pt_regs Struct
+   (Member_plain _r15 tlongu :: 
+    Member_plain _r14 tlongu ::
+    Member_plain _r13 tlongu ::
+    Member_plain _r12 tlongu ::
+    Member_plain _bp tlongu ::
+    Member_plain _bx tlongu ::
+    Member_plain _r11 tlongu ::
+    Member_plain _r10 tlongu ::
+    Member_plain _r9 tlongu ::
+    Member_plain _r8 tlongu ::
+    Member_plain _ax tlongu ::
+    Member_plain _cx tlongu ::
+    Member_plain _dx tlongu ::
+    Member_plain _si tlongu ::
+    Member_plain _di tlongu ::
+    Member_plain _orig_ax tlongu ::
+    Member_plain _ip tlongu :: 
+    Member_plain _flags tlongu ::
+    Member_plain _sp tlongu :: nil)
+    noattr :: nil).
+
+Definition ident_to_string_pt_regs : list (ident * string) := ((_pt_regs, "pt_regs") :: 
+                                                               (_r15, "r15") ::
+                                                               (_r14, "r14") ::
+                                                               (_r13, "r13") ::
+                                                               (_r12, "r12") ::
+                                                               (_bp, "bp") ::
+                                                               (_bx, "bx") ::
+                                                               (_r11, "r11") ::
+                                                               (_r10, "r10") ::
+                                                               (_r9, "r9") ::
+                                                               (_r8, "r8") ::
+                                                               (_ax, "ax") ::
+                                                               (_cx, "cx") ::
+                                                               (_dx, "dx") ::
+                                                               (_si, "si") ::
+                                                               (_di, "di") ::
+                                                               (_orig_ax, "orig_ax") ::
+                                                               (_ip, "ip") ::
+                                                               (_cs, "cs") ::
+                                                               (_flags, "flags") ::
+                                                               (_sp, "sp") ::
+                                                               (_ss, "ss") ::
+                                                               (_ctx, "ctx") :: nil).
+
+Definition _xdp_md : ident := $"xdp_md".
+Definition _data : ident := $"data".
+Definition _data_end : ident := $"data_end".
+Definition _data_meta : ident := $"data_meta".
+Definition _ingress_ifindex : ident := $"ingress_ifindex".
+Definition _rx_queue_index : ident := $"rx_queue_index".
+Definition _egress_ifindex : ident := $"egress_ifindex".
+
+
+Definition ident_to_string_xdp_md : list (ident * string) := ((_xdp_md, "xdp_md") ::
+                                                              (_data, "data") ::
+                                                              (_data_end, "data_end") ::
+                                                              (_data_meta, "data_meta") :: 
+                                                              (_ingress_ifindex, "ingress_ifindex") ::
+                                                              (_rx_queue_index, "rx_queue_index") ::
+                                                              (_egress_ifindex, "egress_ifindex") :: nil).
+
+Definition bcomposites_xdp_md : list bcomposite_definition := 
+(Bcomposite _xdp_md Struct
+   (Member_plain _data tint32u :: 
+    Member_plain _data_end tint32u :: 
+    Member_plain _data_meta tint32u ::
+    Member_plain _ingress_ifindex tint32u :: 
+    Member_plain _rx_queue_index tint32u :: 
+    Member_plain _egress_ifindex tint32u :: nil)
+   noattr :: nil).
+
+
+
+(**** Helper functions ****)
+Definition bpf_get_current_uid_gid : BeePL.external_function
+   := EF_external "bpf_get_current_uid_gid" 
+      {| bsig_args := nil;
+         bsig_ef := nil;
+         bsig_res := tlongu;
+         bsig_cc := cc_default
+      |}.
+
+Definition bpf_map_lookup_elem : BeePL.external_function
+   := EF_external "bpf_map_lookup_elem" 
+      {| bsig_args := (tostruct (ident_of_string "bpf_map") noattr :: tolongu :: nil);
+         bsig_ef := nil;
+         bsig_res := tolongu;
+         bsig_cc := cc_default
+      |}.
+
+Definition bpf_map_update_elem : BeePL.external_function
+   := EF_external "bpf_map_update_elem" 
+      {| bsig_args := (tostruct (ident_of_string "bpf_map") noattr :: trlongu :: trlongu :: tlongu :: nil);
+         bsig_ef := nil;
+         bsig_res := tlongu;
+         bsig_cc := cc_default
+      |}.
+
+
+Definition bpf_get_prandom_u32 : BeePL.external_function
+   := EF_external "bpf_get_prandom_u32" 
+      {| bsig_args := nil;
+         bsig_ef := nil;
+         bsig_res := tint32u;
+         bsig_cc := cc_default
+      |}.
