compiler_test/beepl_test/BeePL_bpf_map_example1.v
@@ -1,0 +1,165 @@
+Require Import Integers AST Ctypes BeePL BeeTypes BeePL_values BeePL_typechecker BeePL_notations BeePL_bpf. 
+From Coq Require Import String ZArith.
+From compcert Require Import Csyntaxdefs.
+Import Csyntaxdefs.CsyntaxNotations.
+Local Open Scope list_scope.
+Local Open Scope string_scope.
+Local Open Scope csyntax_scope.
+
+(*#include <linux/bpf.h>
+#include <bpf/bpf_helpers.h>
+#include <stdint.h>
+#include <stdlib.h>
+#include <memory.h>
+
+// How many times each different user has run programs.
+
+struct {
+    __uint(type, BPF_MAP_TYPE_HASH);
+    __uint(max_entries, 5000000);
+    __type(key, uint64_t);
+    __type(value, uint64_t);
+} counter_table SEC(".maps");
+
+SEC("ksyscall/execve")
+
+int hello(void *ctx) {
+    uint64_t uid;
+    uint64_t counter = 0;
+    uint64_t *p;
+    
+
+    uid = bpf_get_current_uid_gid() & 0xFFFFFFFF;   //returns a 64 bits integer containing the current GID and UID
+                                                    //gets the user id that is running the process that trigegered this krpobe event. 
+                                                    //user-id is held in lowest 32 bits of the 64-bit value that gets returned. (top 32 holds the group id)
+    p = bpf_map_lookup_elem(&counter_table, (&uid)); //returns a pointer to the corresponding value in the hash table 
+    if (p!= 0) {
+        counter = *p;
+    }
+
+    counter++;
+    bpf_map_update_elem(&counter_table, &uid, &counter, 0);
+    return 0;
+}*)
+Definition _val : ident := $"val".
+Definition _counter_table : ident := $"counter_table".
+Definition _uid : ident := $"uid".
+Definition _tuid : ident := $"tuid".
+Definition _counter : ident := $"counter".
+Definition _p : ident := $"p".
+Definition _r : ident := $"r".
+Definition _bpf_get_current_uid_gid : ident := $"bpf_get_current_uid_gid".
+Definition _bpf_map_lookup_elem : ident := $"bpf_map_lookup_elem".
+Definition _bpf_map_update_elem : ident := $"bpf_map_update_elem".
+Definition _ctx : ident := $"ctx".
+Definition _hash_map_example : ident := $"hash_map_example".
+
+Definition ident_to_string : list (ident * string) := ident_to_string_pt_regs ++ 
+                                                      ((_val, "val") ::
+                                                       (_counter_table, "counter_table") ::
+                                                       (_uid, "uid") ::
+                                                       (_tuid, "tuid") ::
+                                                       (_counter, "counter") ::
+                                                       (_p, "p") ::
+                                                       (_r, "r") ::
+                                                       (_bpf_get_current_uid_gid, "_bpf_get_current_uid_gid") ::
+                                                       (_bpf_map_lookup_elem, "_bpf_map_lookup_elem") ::
+                                                       (_bpf_map_update_elem, "_bpf_map_update_elem") ::
+                                                       (_ctx, "ctx") ::
+                                                       (_hash_map_example, "hash_map_example") :: nil).
+                                                 
+
+Definition v_val := {|
+  gvar_info := Maptype (Int.repr 1) 5000000 trlongu trlongu;
+  gvar_init := (Init_int32 (Int.repr 0) :: nil);
+  gvar_readonly := false;
+  gvar_volatile := false
+|}.
+
+Definition v_counter_table := {|
+  gvar_info := (tostruct (ident_of_string "bpf_map") noattr);
+  gvar_init := (Init_addrof _val Ptrofs.zero :: nil);
+  gvar_readonly := false;
+  gvar_volatile := false
+|}.
+
+Definition bcomposites : list bcomposite_definition := bcomposites_pt_regs.
+
+Definition f_hash_map_example : BeePL.function := {| 
+  fn_return := tint32s;
+  fn_effect := Alloc mem_ident :: Alloc mem_ident :: nil;
+  fn_callconv := cc_default;
+  fn_args := (_ctx, tpstruct _pt_regs) :: nil ;
+  fn_vars := ((_uid, trlongu) :: (_tuid, tlongu) :: (_counter, trlongu) :: (_p, tolongu) :: nil); 
+  fn_body := Bind (_uid) trlongu
+               (Prim Ref (clong (Int64.repr 0) tlongu :: nil) (trlongu))
+               (Bind (_counter) trlongu
+                  (Prim Ref (clong (Int64.repr 0) tlongu :: nil) (trlongu))
+                  (Bind (_tuid) tlongu 
+                     (Prim (Bop Cop.Oand) 
+                           (App (Var _bpf_get_current_uid_gid (tfun nil nil tlongu)) nil tlongu ::
+                                 clong (Int64.repr 4294967295) tlongu :: nil) tlongu)
+                     (Bind (_r) trlongu
+                        (Prim Massgn (Var _uid trlongu :: Var _tuid tlongu :: nil) tunit)
+                        (Bind (_r) trlongu 
+                         (Prim Massgn (Var _p tolongu :: 
+                                         App (Var _bpf_map_lookup_elem 
+                                              (tfun (tostruct _counter_table noattr :: tolongu :: nil) nil tolongu)) 
+                                              (Var _counter_table (tostruct (ident_of_string "bpf_map") noattr) ::
+                                               Var _uid trlongu :: nil) tolongu :: nil) tlongu)
+                           (Match (Var _p (tolongu)) 
+                                     (Pnone :: Psome _p :: nil) 
+                                     (cint (Int.repr (-1)%Z) tint32s ::
+                                       (Bind (_r) trlongu 
+                                        (Prim Massgn (Var _counter trlongu ::
+                                                      Prim (Deref) (Var _p (tolongu) :: nil) tlongu :: nil) tlongu)
+                                        (Bind _r tint32s 
+                                           (Bind _r trlongu 
+                                                 (Prim Massgn (Var _counter trlongu ::
+                                                              Prim (Bop Cop.Oadd) (Var _counter tlongu :: clong (Int64.repr 1) tlongu :: nil) tlongu :: nil) tlongu)
+                                                    (App (Var _bpf_map_update_elem 
+                                                         (tfun (tostruct _counter_table noattr :: trlongu :: trlongu :: tlongu :: nil) nil tlongu)) 
+                                                    (Var _counter_table (tostruct (ident_of_string "bpf_map") noattr) ::
+                                                       Var _uid trlongu :: 
+                                                       Var _counter trlongu :: 
+                                                       clong (Int64.repr 0) tlongu :: nil) tlongu) tlongu)
+                                        (cint (Int.repr 0) tint32s) tint32s) tint32s) :: nil) tint32s) tint32s) tint32s) tint32s) tint32s) tint32s;
+                                        
+                                                    
+  is_ebpf := true |}.
+                                                
+
+Definition global_definitions : list (ident * AST.globdef BeePL.fundef type) 
+   := (_counter_table, Gvar v_counter_table) :: (_val, Gvar v_val) :: 
+      (_bpf_get_current_uid_gid, AST.Gfun(BeePL.External (bpf_get_current_uid_gid)
+                                     nil tlongu
+                                     (cc_default))) ::
+      (_bpf_map_lookup_elem, AST.Gfun(BeePL.External (bpf_map_lookup_elem)
+                                     (tostruct (ident_of_string "bpf_map") noattr :: tolongu :: nil) tolongu
+                                     (cc_default))) ::
+      (_bpf_map_update_elem, AST.Gfun(BeePL.External (bpf_map_update_elem)
+                                     (tostruct (ident_of_string "bpf_map") noattr :: trlongu :: trlongu :: tlongu :: nil) tlongu
+                                     (cc_default))) ::
+      (_hash_map_example, AST.Gfun(BeePL.Internal (f_hash_map_example))) :: nil.
+
+Definition public_idents : list ident := (_hash_map_example :: nil).
+
+Lemma bcomposite_correct :
+  wf_bcomposites bcomposites.
+Proof.
+  unfold wf_bcomposites.
+  unfold build_bcomposite_env; simpl; constructor. 
+Qed.
+
+(*Definition example1 : BeePL.program := @mkbprogram bcomposites 
+                                                   global_definitions 
+                                                   public_idents 
+                                                   _hash_map_example 
+                                                   bcomposite_correct
+                                                   ident_to_string.
+
+Compute (type_check_expr example1.(prog_comp_env) 
+                         (bind_vars (bind_vars empty_context f_hash_map_example.(fn_args)) 
+                         f_hash_map_example.(fn_vars)) empty_context f_hash_map_example.(fn_body)).
+
+Compute (type_check_program example1). *) 
